add proofs for encode_instr changes on state

turing_to_while/turing_to_while.thy
@@ -1,8 +1,9 @@
 theory turing_to_while
-  imports Main "Turing" "../IMP-/Com" "../IMP-/Big_StepT" "../IMP-/Small_StepT" "../IMP-/Big_Step_Small_Step_Equivalence" "../fresh_names/Fresh_Class"
+  imports Main "Turing" "../IMP-/Com" "../IMP-/Big_StepT" "../IMP-/Small_StepT" "../IMP-/Big_Step_Small_Step_Equivalence" "../fresh_names/Fresh_Class" "../IMP-/Max_Constant"
 
 begin
 
+subsection "Transformation of the Tape to Natural Numbers and Back"
 type_synonym enc_tape = "nat \<times> nat \<times> nat"
 abbreviation LeftShift_nat:: "nat \<Rightarrow> nat" where
 " LeftShift_nat a \<equiv> a + a"
@@ -20,6 +21,17 @@ value "encode_tape (42, [Oc, Bk, Oc, Oc], [Oc, Bk, Oc, Oc])"
 fun nat_to_tape :: "nat \<Rightarrow> cell list" where
 "nat_to_tape 0 = []" |
 "nat_to_tape n = (if (n mod 2) = 1 then Oc else Bk) # nat_to_tape (n div 2)"
+
+
+lemma nat_to_tape_double[simp]: "n > 0 \<Longrightarrow> nat_to_tape (2 * n) = Bk # (nat_to_tape n)"
+  apply(induct n)
+   apply(auto)
+  done
+
+lemma nat_to_tape_nth_bit: "nat_to_tape (2^n) = replicate n Bk  @ [Oc]"
+  apply(induct n)
+   apply(auto)
+  done
 
 fun decode_tape :: "enc_tape \<Rightarrow> config" where
 "decode_tape (z,n,m) = (z, nat_to_tape n, nat_to_tape m)"
@@ -54,10 +66,8 @@ next
   then show ?case sorry
 qed
 
-lemma tape_to_nat_app_occ: "tape_to_nat (xs @ [Oc]) = 2 ^ (length xs) + tape_to_nat xs"
+lemma nat_to_tape_app_occ: "tape_to_nat(xs @ [Oc]) = 2 ^ (length xs) + tape_to_nat xs"
   sorry
-
-lemma nat_to_tape_app_occ: "2 ^ (length xs) + tape_to_nat xs"
 
 lemma is_cell_list_eq_app_occ[simp]: "is_cell_list_eq (xy @ [Oc]) (xs @ [Oc]) \<longleftrightarrow> (xy @ [Oc]) = (xs @ [Oc])"
   by simp
@@ -78,74 +88,206 @@ next
   next
     case Oc
     from "snoc.IH" have "is_cell_list_eq (nat_to_tape (tape_to_nat (xs @ [Oc]))) (xs @ [Oc])"
-    then show ?thesis sorry
+    then show ?thesis try
 
   qed
 qed
 lemma encode_decode_inverse: "(z,x,y) = encode_tape(decode_tape(z,x,y))"
   sorry
 
-definition LeftShift:: "atomExp \<Rightarrow> aexp" ("_\<lless>") where
-"LeftShift a = Plus a a"
-definition encode_tape_instr :: "action  \<Rightarrow> com" where
+
+
+subsection "Encoding of Tape Instructions As arithmetic Operations"
+
+abbreviation LeftShift:: "atomExp \<Rightarrow> aexp" ("_\<lless>") where
+"LeftShift a \<equiv> Plus a a"
+fun encode_tape_instr :: "action  \<Rightarrow> com" where
 "encode_tape_instr a = (case a of Nop \<Rightarrow> SKIP |
                                   W0 \<Rightarrow> ''y''::= (V ''y''\<then>);;''y''::= (V ''y''\<lless>) |
                                   W1 \<Rightarrow> ''y''::= (V ''y''\<then>);;''y''::=(V ''y''\<lless>);;''y''::= ((V ''y'') \<oplus> (N 1)) |
                                   L \<Rightarrow> ''y''::= (V ''y''\<lless>);;''t''::=(V ''x''\<doteq>1);;''y''::= ((V ''y'') \<oplus> (V ''t''));; ''x''::= (V ''x''\<then>) |
                                   R \<Rightarrow>''x''::= (V ''x''\<lless>);;''t''::=(V ''y''\<doteq>1);;''x''::= ((V ''x'') \<oplus> (V ''t''));;''y''::= (V ''y''\<then>))"
 
+lemma rightShift_state: 
+  assumes rightShift_com: "(v::= (V v\<then>), s) \<Rightarrow>\<^bsup> k \<^esup> s'"
+  shows " s(v := s v div 2) = s'" 
+  using assms proof -
+   show ?thesis using rightShift_com by auto
+ qed
+
+lemma rightShift_state_: 
+  assumes rightShift_com: "(v::= (V v\<then>), s) \<Rightarrow>\<^bsup> k \<^esup> s'"
+  shows " (s v) div 2 = s' v" 
+  using assms proof -
+   show ?thesis using rightShift_com by auto
+ qed
+
+lemma encode_w0_x: 
+  assumes encode_w0: "(c;;(encode_tape_instr W0),s0) \<Rightarrow>\<^bsup> k \<^esup> s"
+    and encode_instr: "(c,s0) \<Rightarrow>\<^bsup> k' \<^esup> s'"
+shows "s ''x'' = s' ''x''"
+  using assms proof -
+  obtain k' s1 k'' where "(c,s0) \<Rightarrow>\<^bsup> k' \<^esup> s1" and
+         "(encode_tape_instr W0,s1) \<Rightarrow>\<^bsup> k'' \<^esup> s" using encode_w0 by blast 
+  then have "s1 = s'" using big_step_t_determ2 encode_instr by blast
+  have "''x'' \<notin> set (Max_Constant.all_variables (encode_tape_instr W0))" by simp
+  then show ?thesis
+    by (metis \<open>(encode_tape_instr W0, s1) \<Rightarrow>\<^bsup> k'' \<^esup> s\<close> \<open>s1 = s'\<close> com_only_vars)
+qed
+
+lemma encode_w0_y: 
+  assumes encode_w0: "(c;;(encode_tape_instr W0),s0) \<Rightarrow>\<^bsup> k \<^esup> s"
+    and encode_instr: "(c,s0) \<Rightarrow>\<^bsup> k' \<^esup> s'"
+shows "s ''y'' = (if even (s' ''y'') then s' ''y'' else s' ''y'' - 1)"
+  using assms proof -
+  obtain k' s1 k'' where "(c,s0) \<Rightarrow>\<^bsup> k' \<^esup> s1" and
+         "(encode_tape_instr W0,s1) \<Rightarrow>\<^bsup> k'' \<^esup> s" and
+         "k'' = 4" using encode_w0 by fastforce
+  then have "s1 = s'" using big_step_t_determ2 encode_instr by blast
+  have "k' + k'' = k"
+    by (meson Seq \<open>(c, s0) \<Rightarrow>\<^bsup> k' \<^esup> s1\<close> \<open>(encode_tape_instr W0, s1) \<Rightarrow>\<^bsup> k'' \<^esup> s\<close> big_step_t_determ2 encode_w0)
+  from encode_w0 have "(c;;''y''::= (V ''y''\<then>);;''y''::= (V ''y''\<lless>),s0) \<Rightarrow>\<^bsup> k \<^esup> s" by fastforce
+  have "(c;;''y''::= (V ''y''\<then>);;''y''::= Plus (V ''y'') (V ''y''),s0) \<Rightarrow>\<^bsup> k \<^esup> s1(''y'' := LeftShift_nat (s1 ''y'' div 2))" 
+    apply(rule Seq) apply(rule Seq) apply(auto) apply(fact) apply(rule AssignI) using \<open>k' + k'' = k\<close> \<open>k'' = 4\<close> by auto
+  then show ?thesis by (metis \<open>(c;; ''y'' ::= (V ''y''\<then>);; ''y'' ::= V ''y''\<lless>, s0) \<Rightarrow>\<^bsup> k \<^esup> s\<close> \<open>s1 = s'\<close> big_step_t_determ2 dvd_mult_div_cancel fun_upd_same mult_2 odd_two_times_div_two_nat)
+qed
+
+lemma encode_w1_x: 
+  assumes encode_w1: "(c;;(encode_tape_instr W1),s0) \<Rightarrow>\<^bsup> k \<^esup> s"
+    and encode_instr: "(c,s0) \<Rightarrow>\<^bsup> k' \<^esup> s'"
+shows "s ''x'' = s' ''x''"
+  using assms proof -
+  obtain k' s1 k'' where "(c,s0) \<Rightarrow>\<^bsup> k' \<^esup> s1" and
+         "(encode_tape_instr W1,s1) \<Rightarrow>\<^bsup> k'' \<^esup> s" using encode_w1 by blast 
+  then have "s1 = s'" using big_step_t_determ2 encode_instr by blast
+  have "''x'' \<notin> set (Max_Constant.all_variables (encode_tape_instr W1))" by simp                         
+  then show ?thesis
+    by (metis \<open>(encode_tape_instr W1, s1) \<Rightarrow>\<^bsup> k'' \<^esup> s\<close> \<open>s1 = s'\<close> com_only_vars)
+qed
+
+lemma encode_w1_y: (* also provable by showing it is simply Suc W0 *)
+  assumes encode_w1: "(c;;(encode_tape_instr W1),s0) \<Rightarrow>\<^bsup> k \<^esup> s"
+    and encode_instr: "(c,s0) \<Rightarrow>\<^bsup> k' \<^esup> s'"
+shows "s ''y'' = (if even (s' ''y'') then s' ''y'' + 1 else s' ''y'')"
+  using assms proof -
+  obtain k' s1 k'' where "(c,s0) \<Rightarrow>\<^bsup> k' \<^esup> s1" and
+         "(encode_tape_instr W1,s1) \<Rightarrow>\<^bsup> k'' \<^esup> s" and
+         "k'' = 6" using encode_w1 by fastforce
+  then have "s1 = s'" using big_step_t_determ2 encode_instr by blast
+  have "k' + k'' = k"
+    by (meson Seq \<open>(c, s0) \<Rightarrow>\<^bsup> k' \<^esup> s1\<close> \<open>(encode_tape_instr W1, s1) \<Rightarrow>\<^bsup> k'' \<^esup> s\<close> big_step_t_determ2 encode_w1)
+  from encode_w1 have "(c;;''y''::= (V ''y''\<then>);;''y''::= (V ''y''\<lless>);;''y''::= ((V ''y'') \<oplus> (N 1)),s0) \<Rightarrow>\<^bsup> k \<^esup> s" by fastforce
+  have "(c;;''y''::= (V ''y''\<then>);;''y''::= Plus (V ''y'') (V ''y'');;''y''::= ((V ''y'') \<oplus> (N 1)),s0) \<Rightarrow>\<^bsup> k \<^esup>s1(''y'' := Suc (LeftShift_nat (s1 ''y'' div 2)))" 
+    apply(rule Seq) apply(rule Seq) apply(rule Seq) apply(auto) apply(fact) apply(rule AssignI) using \<open>k' + k'' = k\<close> \<open>k'' = 6\<close> by auto
+  then show ?thesis
+    by (smt (verit, del_insts) Suc_eq_plus1 \<open>(c;; ''y'' ::= (V ''y''\<then>);; ''y'' ::= V ''y''\<lless>;; ''y'' ::= (V ''y'' \<oplus> N 1), s0) \<Rightarrow>\<^bsup> k \<^esup> s\<close> \<open>s1 = s'\<close> add_self_div_2 bigstep_det bit_eq_rec even_add even_succ_div_2 fun_upd_same odd_one plus_1_eq_Suc)
+  qed
+
+
+lemma encode_L_x: 
+  assumes encode_L: "(c;;(encode_tape_instr L),s0) \<Rightarrow>\<^bsup> k \<^esup> s"
+    and encode_instr: "(c,s0) \<Rightarrow>\<^bsup> k' \<^esup> s'"
+shows "s ''x'' = s' ''x'' div 2"
+  using assms proof -
+  obtain k' s1 k'' where "(c,s0) \<Rightarrow>\<^bsup> k' \<^esup> s1" and
+         "(encode_tape_instr L,s1) \<Rightarrow>\<^bsup> k'' \<^esup> s" and
+         "k'' = 8" using encode_L by fastforce
+  then have "s1 = s'" using big_step_t_determ2 encode_instr by blast
+  have "k' + k'' = k"
+    by (meson Seq \<open>(c, s0) \<Rightarrow>\<^bsup> k' \<^esup> s1\<close> \<open>(encode_tape_instr L, s1) \<Rightarrow>\<^bsup> k'' \<^esup> s\<close> big_step_t_determ2 encode_L)
+  from encode_L have "(c;;''y''::= (V ''y''\<lless>);;''t''::=(V ''x''\<doteq>1);;''y''::= ((V ''y'') \<oplus> (V ''t''));; ''x''::= (V ''x''\<then>),s0) \<Rightarrow>\<^bsup> k \<^esup> s" by fastforce
+  have "(c;;''y''::= (V ''y''\<lless>);;''t''::=(V ''x''\<doteq>1);;''y''::= ((V ''y'') \<oplus> (V ''t''));; ''x''::= (V ''x''\<then>),s0) \<Rightarrow>\<^bsup> k \<^esup>  s1
+    (''t'' := s1 ''x'' mod 2, ''y'' := LeftShift_nat (s1 ''y'') + s1 ''x'' mod 2,
+     ''x'' := aval (V ''x''\<then>) (s1(''t'' := s1 ''x'' mod 2, ''y'' := LeftShift_nat (s1 ''y'') + s1 ''x'' mod 2)))"
+    apply(rule Seq) apply(rule Seq) apply(rule Seq) apply(rule Seq) apply(auto) apply(fact) apply(rule AssignI) using \<open>k' + k'' = k\<close> \<open>k'' = 8\<close> by auto
+  then show ?thesis
+    by (smt (z3) \<open>(c;; ''y'' ::= V ''y''\<lless>;; ''t'' ::= (V ''x'' \<doteq>1);; ''y'' ::= (V ''y'' \<oplus> V ''t'');; ''x'' ::= (V ''x''\<then>), s0) \<Rightarrow>\<^bsup> k \<^esup> s\<close> \<open>s1 = s'\<close> atomVal.simps(1) aval.simps(5) big_step_t_determ2 char.inject fun_upd_other fun_upd_same list.inject)
+qed
+
+lemma encode_L_y: 
+  assumes encode_L: "(c;;(encode_tape_instr L),s0) \<Rightarrow>\<^bsup> k \<^esup> s"
+    and encode_instr: "(c,s0) \<Rightarrow>\<^bsup> k' \<^esup> s'"
+  shows"s ''y'' = (if even (s' ''x'') then s' ''y'' * 2 else  s' ''y'' * 2 + 1)"
+  using assms proof -
+  obtain k' s1 k'' where "(c,s0) \<Rightarrow>\<^bsup> k' \<^esup> s1" and
+         "(encode_tape_instr L,s1) \<Rightarrow>\<^bsup> k'' \<^esup> s" and
+         "k'' = 8" using encode_L by fastforce
+  then have "s1 = s'" using big_step_t_determ2 encode_instr by blast
+  have "k' + k'' = k"
+    by (meson Seq \<open>(c, s0) \<Rightarrow>\<^bsup> k' \<^esup> s1\<close> \<open>(encode_tape_instr L, s1) \<Rightarrow>\<^bsup> k'' \<^esup> s\<close> big_step_t_determ2 encode_L)
+  from encode_L have "(c;;''y''::= (V ''y''\<lless>);;''t''::=(V ''x''\<doteq>1);;''y''::= ((V ''y'') \<oplus> (V ''t''));; ''x''::= (V ''x''\<then>),s0) \<Rightarrow>\<^bsup> k \<^esup> s" by fastforce
+  have "(c;;''y''::= (V ''y''\<lless>);;''t''::=(V ''x''\<doteq>1);;''y''::= ((V ''y'') \<oplus> (V ''t''));; ''x''::= (V ''x''\<then>),s0) \<Rightarrow>\<^bsup> k \<^esup>  s1
+    (''t'' := s1 ''x'' mod 2, ''y'' := LeftShift_nat (s1 ''y'') + s1 ''x'' mod 2,
+     ''x'' := aval (V ''x''\<then>) (s1(''t'' := s1 ''x'' mod 2, ''y'' := LeftShift_nat (s1 ''y'') + s1 ''x'' mod 2)))"
+    apply(rule Seq) apply(rule Seq) apply(rule Seq) apply(rule Seq) apply(auto) apply(fact) apply(rule AssignI) using \<open>k' + k'' = k\<close> \<open>k'' = 8\<close> by auto
+  then show ?thesis sorry
+  qed
+
+
+
+
+subsection "Transforming Turing Machine to IMP-"
+
 abbreviation nth_name:: "nat \<Rightarrow> string" where
 "nth_name n \<equiv> (as_string ((next^^n) (default::name)))"
 
 
-fun turing_to_while :: "config \<Rightarrow> tprog0 \<Rightarrow> name \<Rightarrow> com" where (* state has to evaluate all variables to 1 except (next (default::name)) which has to be 0 at the beginning *)
-"turing_to_while c [] _ = (let (z,x,y) = encode_tape c in (''z''::=A (N z);;''x''::=A (N x);;''y''::=A (N y)));;
-                                          WHILE (as_string (default::name))\<noteq>0 DO SKIP" |
-"turing_to_while c ((a0,s0)#(a1,s1)#is) n = turing_to_while c is (next n);;
+fun turing_to_while_acc :: "tprog0 \<Rightarrow> name \<Rightarrow> com" where (* state has to evaluate all variables to 1 except (next (default::name)) which has to be 0 at the beginning *)
+"turing_to_while_acc [] _ = SKIP" |
+"turing_to_while_acc ((a0,s0)#(a1,s1)#is) n = turing_to_while_acc is (next n);;
   IF (as_string n)\<noteq>0 THEN SKIP
                      ELSE (''t''::=(V ''x''\<doteq>1);;IF ''t''\<noteq>0 THEN 
-                            encode_tape_instr a1;;(nth_name s1)::=A (N 0);;(as_string n)::=A (N 1)
-                          ELSE encode_tape_instr a0;;(nth_name s0)::=A (N 0);;(as_string n)::=A (N 1)) "
+                            encode_tape_instr a1;;(nth_name s1)::=A (N 0);;(as_string n)::=A (N 1);;''z''::=(A(N s1))
+                          ELSE encode_tape_instr a0;;(nth_name s0)::=A (N 0);;(as_string n)::=A (N 1));;''z''::=(A(N s0)) "
+
+fun turing_to_while :: "config \<Rightarrow> tprog0 \<Rightarrow> com" where
+"turing_to_while c p = (let (z,x,y) = encode_tape c in (''z''::=A (N z);;''x''::=A (N x);;''y''::=A (N y)));;
+                                          WHILE (as_string (default::name))\<noteq>0 DO turing_to_while_acc p (next default)"
 
 
-
-lemma update_passthrough_nop[simp]: "turing_to_while (s,update Nop (l,r)) p (next default) = turing_to_while (s,l,r) p (next default)"
+lemma update_passthrough_nop[simp]: "turing_to_while (s,update Nop (l,r)) p = turing_to_while (s,l,r) p"
   by simp
 lemma update_state_nop[simp]: 
-  assumes tm_conversion: "(turing_to_while (q,l,r) p (next default),\<lambda>s. if s = nth_name q then 0 else 1) \<Rightarrow>\<^bsup> k \<^esup> s"
-    and tm_nop_conversion: "(turing_to_while (q,update Nop (l,r)) p (next default),\<lambda>s. if s = nth_name q then 0 else 1) \<Rightarrow>\<^bsup> k \<^esup> s'"
+  assumes tm_conversion: "(turing_to_while (q,l,r) p,\<lambda>s. if s = nth_name q then 0 else 1) \<Rightarrow>\<^bsup> k \<^esup> s"
+    and tm_nop_conversion: "(turing_to_while (q,update Nop (l,r)) p,\<lambda>s. if s = nth_name q then 0 else 1) \<Rightarrow>\<^bsup> k \<^esup> s'"
   shows "s = s'"
 proof -
-  from tm_conversion have "(turing_to_while (q,l,r) p (next default),\<lambda>s. if s = nth_name q then 0 else 1) \<Rightarrow>\<^bsup> k \<^esup> s" by simp
-  then have "(turing_to_while (q,update Nop (l,r)) p (next default),\<lambda>s. if s = nth_name q then 0 else 1) \<Rightarrow>\<^bsup> k \<^esup> s" by simp
+  from tm_conversion have "(turing_to_while (q,l,r) p,\<lambda>s. if s = nth_name q then 0 else 1) \<Rightarrow>\<^bsup> k \<^esup> s" by simp
+  then have "(turing_to_while (q,update Nop (l,r)) p,\<lambda>s. if s = nth_name q then 0 else 1) \<Rightarrow>\<^bsup> k \<^esup> s" by simp
   thus ?thesis using bigstep_det tm_nop_conversion by auto
 qed
-lemma update_passthrough_w0[simp]: "turing_to_while (s,update W0 (l,r)) p (next default) = turing_to_while (s,l,Bk#(tl r)) p (next default)"
+lemma update_passthrough_w0[simp]: "turing_to_while (s,update W0 (l,r)) p = turing_to_while (s,l,Bk#(tl r)) p"
   by simp
-lemma update_state_w0[simp]: 
-  assumes tm_conversion: "(turing_to_while (q,l,r) p (next default),\<lambda>s. if s = nth_name q then 0 else 1) \<Rightarrow>\<^bsup> k \<^esup> s"
-    and tm_nop_conversion: "(turing_to_while (q,update W0 (l,r)) p (next default),\<lambda>s. if s = nth_name q then 0 else 1) \<Rightarrow>\<^bsup> k' \<^esup> s'"
-  shows "s ''z'' = s' ''z''" (* \<and> s ''x'' = s' ''x'' \<and> s ''y'' \<ge> s' ''y''" *)
-proof(induct "q l r p" rule: turing_to_while.induct)
+lemma update_state_w0[simp]:  
+  assumes tm_wf: "tm_wf (p,1)"
+  and tm_conversion: "(turing_to_while (q,l,r) p,\<lambda>s. if s = nth_name q then 0 else 1) \<Rightarrow>\<^bsup> k \<^esup> s"
+  and tm_nop_conversion: "(turing_to_while (q,update W0 (l,r)) p,\<lambda>s. if s = nth_name q then 0 else 1) \<Rightarrow>\<^bsup> k' \<^esup> s'"
+  shows "s ''x'' = s' ''x''" (* \<and> s ''x'' = s' ''x'' \<and> s ''y'' \<ge> s' ''y''" *)
+using assms proof(induct p arbitrary: k k')
+  case Nil
+  then show ?case by simp
+next
+  case (Cons a p)
+  then show ?case by auto
 qed
-lemma update_passthrough_w1[simp]: "turing_to_while (s,update W1 (l,r)) p (next default) = turing_to_while (s,l,Oc#(tl r)) p (next default)"
+lemma update_passthrough_w1[simp]: "turing_to_while (s,update W1 (l,r)) p  = turing_to_while (s,l,Oc#(tl r)) p"
   by simp
-lemma update_passthrough_L[simp]: "turing_to_while (s,update L (l,r)) p (next default) = turing_to_while (s,tl l,if l=[] then Bk# r else (hd l)#r) p (next default)"
+lemma update_passthrough_L[simp]: "turing_to_while (s,update L (l,r)) p = turing_to_while (s,tl l,if l=[] then Bk# r else (hd l)#r) p"
   by simp
-lemma update_passthrough_R[simp]: "turing_to_while (s,update R (l,r)) p (next default) = turing_to_while (s,if r=[] then Bk# l else (hd r)#l, tl r) p (next default)"
+lemma update_passthrough_R[simp]: "turing_to_while (s,update R (l,r)) p = turing_to_while (s,if r=[] then Bk# l else (hd r)#l, tl r) p"
   by simp
 
 
 lemma conversion_step_correct: 
   assumes tm_wf: "tm_wf (p,1)"
-  and "(turing_to_while (state,l,r) p (next default), \<lambda>s. if s = nth_name state then 0 else 1) \<Rightarrow>\<^bsup> k \<^esup> s " 
+  and "(turing_to_while (state,l,r) p, \<lambda>s. if s = nth_name state then 0 else 1) \<Rightarrow>\<^bsup> k \<^esup> s " 
   and "encode_tape (step0 c p) = (s1,l1,r1)"
   shows "(l1,r1) = (s ''x'', s ''y'') \<and> s (nth_name state) = 0"
   sorry
 lemma conversion_correct:
   assumes tm_wf: "tm_wf (p,0)"
   and tm_accepts: "is_final(steps0 c p n)"
-  and "(turing_to_while c p (next default), \<lambda>s. if s = ''__'' then 0 else 1) \<Rightarrow>\<^bsup> k \<^esup> s " 
+  and "(turing_to_while c p, \<lambda>s. if s = ''__'' then 0 else 1) \<Rightarrow>\<^bsup> k \<^esup> s " 
   shows "encode_tape (steps0 c p n) = (s ''_'',s ''x'', s ''y'')"
   using assms proof (induct p)
       case Nil
